function up to injective

Astlib/Basic/SetOperation/Function.lean
@@ -2,26 +2,42 @@ import Astlib.Basic.SetOperation.Relation
 
 namespace FirstOrder.Language.MemStructure
 
+section Basic
+
 variable {M : MemStructure} (x y z x₁ x₂ y₁ y₂ u v : M)
 
 def IsFunction (f : M) :=
   IsRelation f ∧ ∀ ⦃x y₁ y₂ : M⦄, x [f] y₁ → x [f] y₂ → y₁ = y₂
 
+@[simp, grind .]
 theorem IsFunction.isRelation {f : M} (hf : IsFunction f) : IsRelation f := hf.left
 
-@[simp, grind! .]
+@[simp, grind .]
 theorem IsFunction.eq
     {f x y₁ y₂: M} (hf : IsFunction f) (h₁ : x [f] y₁) (h₂ : x [f] y₂) : y₁ = y₂ := by
   grind [IsFunction]
 
-@[simp]
-theorem empty_isFunction [M.HasEmpty] : IsFunction (∅ : M) := by
+@[simp, grind .]
+theorem isFunction_empty [M.HasEmpty] : IsFunction (∅ : M) := by
   simp [IsFunction]
 
+@[simp, grind .]
 theorem IsFunction.subset {f g : M} (hf : IsFunction f) (hgf : g ⊆ f) :
     IsFunction g := by
   simp only [IsFunction, hf.isRelation.subset hgf, true_and]
   exact fun x y₁ y₂ h₁ h₂ ↦ hf.eq (hgf h₁) (hgf h₂)
+
+theorem IsFunction.inter_right [M.ClosedUnderDeltaZeroComprehension]
+    {f g : M} (hf : IsFunction f) : IsFunction (f ∩ g) := by
+  grind
+
+theorem IsFunction.inter_left [M.ClosedUnderDeltaZeroComprehension]
+    {f g : M} (hg : IsFunction g) : IsFunction (f ∩ g) := by
+  grind
+
+theorem IsFunction.sdiff [M.ClosedUnderDeltaZeroComprehension]
+    {f g : M} (hf : IsFunction f) : IsFunction (f \ g) := by
+  grind
 
 noncomputable instance (f x : M) : Decidable (∃ y, x [f] y) :=
   Classical.propDecidable _
@@ -47,7 +63,7 @@ theorem IsFunction.exists_val
 variable [M.ClosedUnderDeltaZeroComprehension]
     [M.ClosedUnderSUnion] [M.Extensional] [M.ClosedUnderPair]
 
-@[simp]
+-- @[simp]
 theorem rel_val
     {f x : M} (hx : x ∈ dom f) : x [f] (f ﹫ x) := by
   grind [val]
@@ -74,6 +90,7 @@ theorem IsFunction.mem_dom_iff {f : M} (x : M) (hf : IsFunction f) :
     x ∈ dom f ↔ x [f] (f ﹫ x) := by
   grind
 
+@[grind =]
 theorem IsFunction.mem_ran_iff {f : M} (y : M) (hf : IsFunction f) :
     y ∈ ran f ↔ ∃ x ∈ dom f, f ﹫ x = y := by
   rw [M.mem_ran_iff]
@@ -83,13 +100,48 @@ theorem IsFunction.subset_dom_sprod_ran [M.ClosedUnderSProd] {f : M} (hf : IsFun
     f ⊆ dom f ×ˢ ran f :=
   hf.isRelation.subset_dom_sprod_ran
 
-@[grind! .]
-theorem IsFunction.isFunction_comp [M.ClosedUnderSProd]
+def FunctionAgree (f g : M) := ∀ ⦃x⦄, x ∈ dom f ∩ dom g → f ﹫ x = g ﹫ x
+
+@[simp, grind .]
+theorem IsFunction.union {f g : M}
+    (hf : IsFunction f) (hg : IsFunction g)
+    (hfg : FunctionAgree f g) : IsFunction (f ∪ g) := by
+  refine ⟨hf.isRelation.union hg.isRelation, fun x y₁ y₂ h₁ h₂ ↦ ?_⟩
+  rw [mem_union] at h₁ h₂
+  rcases h₁ with h₁ | h₁
+  · rcases h₂ with h₂ | h₂
+    · grind
+    · grind [hfg (x := x) (by grind)]
+  · rcases h₂ with h₂ | h₂
+    · grind [hfg (x := x) (by grind)]
+    · grind
+
+@[simp, grind .]
+theorem IsFunction.sUnion {X : M}
+    (hX₁ : ∀ f ∈ X, IsFunction f)
+    (hX₂ : ∀ f ∈ X, ∀ g ∈ X, FunctionAgree f g) : IsFunction (⋃₀ X) := by
+  refine ⟨IsRelation.sUnion (fun f hf ↦ (hX₁ f hf).isRelation), fun x y₁ y₂ h₁ h₂ ↦ ?_⟩
+  simp only [mem_sUnion_iff] at h₁ h₂
+  obtain ⟨f, hf₁, hf₂⟩ := h₁
+  obtain ⟨g, hg₁, hg₂⟩ := h₂
+  grind [(hX₁ f hf₁).union (hX₁ g hg₁) (by grind)]
+
+end Basic
+
+section Comp
+
+variable {M : MemStructure} (x y z x₁ x₂ y₁ y₂ u v : M)
+
+variable [M.Extensional] [M.ClosedUnderPair] [M.ClosedUnderSProd]
+  [M.ClosedUnderDeltaZeroComprehension] [M.ClosedUnderSUnion]
+
+@[grind .]
+theorem IsFunction.isFunction_comp
     {f g : M} (hf : IsFunction f) (hg : IsFunction g) : IsFunction (f !∘ g) := by
   grind [IsFunction]
 
 @[grind .]
-theorem mem_dom_comp [M.ClosedUnderSProd]
+theorem mem_dom_comp
     {f g x : M} (hf : IsFunction f) (hg : IsFunction g)
     (hx : x ∈ dom g) (hx' : g ﹫ x ∈ dom f) :
     x ∈ dom (f !∘ g) := by
@@ -97,37 +149,147 @@ theorem mem_dom_comp [M.ClosedUnderSProd]
   rw [hf.mem_dom_iff] at hx'
   grind
 
+@[grind .]
+theorem dom_comp
+    {f g : M} (hf : IsFunction f)
+    (h : ran g ⊆ dom f) :
+    dom g = dom (f !∘ g) := by
+  ext x
+  constructor
+  · simp only [mem_dom_iff, rel_comp]
+    intro ⟨y, hy⟩
+    exact ⟨f ﹫ y, y, hy, by grind [show y ∈ ran g by grind]⟩
+  · grind
+
 @[grind =]
-theorem val_comp [M.ClosedUnderSProd]
+theorem val_comp
     {f g x : M} (hf : IsFunction f) (hg : IsFunction g)
     (hx : x ∈ dom g) (hx' : g ﹫ x ∈ dom f) :
     (f !∘ g) ﹫ x = f ﹫ (g ﹫ x) := by
   rw [hg.mem_dom_iff] at hx
   rw [hf.mem_dom_iff] at hx'
   grind
-  -- suffices ((∃ u ∈ dom S, ∃ v ∈ ran R, z = !(u, v)) ∧
-  --   ∃ x x_1, (x [S] x_1) ∧ ∃ x_2 x_3, (x_1 [R] x_3) ∧ (∃ x_4, z = !(x, x_4)) ∧ z = !(x_2, x_3))
-  --   ↔ ∃ a b c, z = !(a, c) ∧ (a [S] b) ∧ (b [R] c) by
-  --   simpa [MemStructure.comp, mem_comprehension_iff]
-  -- refine ⟨by grind, fun ⟨a, b, c, hz, hab, hbc⟩ ↦ ?_⟩
-  -- exact ⟨⟨a, by grind, c, by grind, hz⟩, ⟨a, b, hab, a, c, hbc, ⟨⟨c, hz⟩, hz⟩⟩⟩
 
+end Comp
 
--- theorem dom_comp_subset [M.Extensional] [M.ClosedUnderPair] [M.ClosedUnderSProd] (R S : M) :
---     dom (R !∘ S) ⊆ dom S := by
---   grind
+section Id
 
--- theorem ran_comp_subset [M.Extensional] [M.ClosedUnderPair] [M.ClosedUnderSProd] (R S : M) :
---     ran (R !∘ S) ⊆ ran R := by
---   grind
+variable {M : MemStructure} (x y z x₁ x₂ y₁ y₂ u v : M)
 
+variable [M.Extensional] [M.ClosedUnderPair] [M.ClosedUnderSProd]
+  [M.ClosedUnderDeltaZeroComprehension]
 
-omit [M.ClosedUnderSUnion] in
-theorem id_isFunction [M.ClosedUnderSProd]
+@[simp, grind .]
+theorem isFunction_id
     (a : M) : IsFunction (id a) := by
   grind [IsFunction, id]
 
+@[simp, grind =]
+theorem id_val (a : M) {x : M} (hx : x ∈ a) : id a ﹫ x = x :=
+  (isFunction_id _).val_eq_of_rel (by grind)
 
+@[simp, grind =]
+theorem IsFunction.comp_id [M.ClosedUnderSUnion]
+    {f a : M} (hf : IsFunction f) (h : dom f ⊆ a) :
+    f !∘ (id a) = f := by
+  grind [IsFunction]
+
+@[simp, grind =]
+theorem IsFunction.id_comp [M.ClosedUnderSUnion]
+    {f a : M} (hf : IsFunction f) (h : ran f ⊆ a) :
+    (id a) !∘ f = f := by
+  grind [IsFunction]
+
+end Id
+
+section IsFunctionFromTo
+
+variable {M : MemStructure} (x y z x₁ x₂ y₁ y₂ u v : M)
+
+def IsFunctionFrom (f a : M) := IsFunction f ∧ dom f = a
+
+@[simp, grind .]
+theorem isFunctionFrom_dom {f : M} (hf : IsFunction f) : IsFunctionFrom f (dom f) := by
+  simp [IsFunctionFrom, hf]
+
+@[simp, grind .]
+theorem isFunctionFrom_empty [M.HasEmpty] [M.Extensional] [M.ClosedUnderSUnion] [M.ClosedUnderPair]
+  [M.ClosedUnderDeltaZeroComprehension] : IsFunctionFrom (∅ : M) ∅ := by
+  simp [IsFunctionFrom]
+
+def IsFunctionTo (f b : M) := IsFunction f ∧ ran f ⊆ b
+
+@[simp, grind .]
+theorem isFunctionTo_mono {f b b' : M} (hfb : IsFunctionTo f b) (hbb' : b ⊆ b') :
+    IsFunctionTo f b' := by
+  grind [IsFunctionTo]
+
+@[simp, grind .]
+theorem isFunctionTo_ran {f : M} (hf : IsFunction f) :
+    IsFunctionTo f (ran f) := by
+  grind [IsFunctionTo]
+
+@[simp, grind .]
+theorem isFunctionTo_empty [M.HasEmpty] [M.Extensional] [M.ClosedUnderSUnion] [M.ClosedUnderPair]
+    [M.ClosedUnderDeltaZeroComprehension] (b : M) : IsFunctionTo (∅ : M) b := by
+  have : IsFunctionTo (∅ : M) ∅ := by grind [IsFunctionTo]
+  grind
+
+def IsFunctionFromTo (f a b : M) := IsFunctionFrom f a ∧ IsFunctionTo f b
+
+notation:50 f " !: " a:50 " → " b:50 => IsFunctionFromTo f a b
+
+theorem isFunctionFromTo_iff (f a b : M) :
+    f !: a → b ↔ IsFunction f ∧ dom f = a ∧ ran f ⊆ b := by
+  grind [IsFunctionFromTo, IsFunctionFrom, IsFunctionTo]
+
+@[simp, grind .]
+theorem isFunctionFromTo_mono {f a b b' : M} (hf : f !: a → b) (hbb' : b ⊆ b') :
+    f !: a → b' := by
+  grind [IsFunctionFromTo]
+
+@[simp, grind .]
+theorem isFunctionFromTo_dom_ran {f : M} (hf : IsFunction f) :
+    f !: dom f → ran f := by
+  grind [IsFunctionFromTo]
+
+@[simp, grind .]
+theorem isFunctionFromTo_empty [M.HasEmpty] [M.Extensional] [M.ClosedUnderSUnion]
+    [M.ClosedUnderPair]
+    [M.ClosedUnderDeltaZeroComprehension] (b : M) : ∅ !: ∅ → b := by
+  grind [IsFunctionFromTo]
+
+@[simp, grind .]
+theorem IsFunctionFromTo.comp [M.HasEmpty] [M.Extensional] [M.ClosedUnderSUnion]
+    [M.ClosedUnderPair]
+    [M.ClosedUnderDeltaZeroComprehension] [M.ClosedUnderSProd]
+    {f g a b c : M} (hf : f !: a → b) (hg : g !: b → c) :
+    g !∘ f !: a → c := by
+  grind [isFunctionFromTo_iff, ran_comp_subset]
+
+end IsFunctionFromTo
+
+section Injective
+
+variable {M : MemStructure} (x y z x₁ x₂ y₁ y₂ u v : M)
+
+variable [M.Extensional] [M.ClosedUnderSUnion] [M.ClosedUnderPair]
+  [M.ClosedUnderDeltaZeroComprehension]
+
+def IsInjective (f : M) := ∀ ⦃x y⦄, x ∈ dom f → y ∈ dom f → f ﹫ x = f ﹫ y → x = y
+
+@[simp, grind .]
+theorem isInjective_empty [M.HasEmpty] : IsInjective (∅ : M) := by
+  grind [IsInjective]
+
+theorem isInjective_iff_isFunction_inv [M.ClosedUnderSProd] {f : M} (hf : IsFunction f) :
+    IsInjective f ↔ IsFunction (f⁻¹) := by
+  refine ⟨fun h ↦ ⟨by grind, by intros; exact h (by grind) (by grind) (by grind)⟩, ?_⟩
+  intro h y₁ y₂ h₁ h₂ h₁₂
+  let x := f ﹫ y₁
+  grind [show x [f⁻¹] y₁ by grind, show x [f⁻¹] y₂ by grind]
+
+end Injective
 -- @[grind =]
 -- theorem mem_inv [M.Extensional] [M.ClosedUnderPair] [M.ClosedUnderSProd]
 --     (R z : M) :
